* Update all property definitions, add some documentation

src/aadl_dynamic_thread.v
@@ -23,10 +23,15 @@ Require Import Oqarina.properties.properties.
 Require Import Oqarina.aadl_categories.
 Require Import Oqarina.aadl.
 Require Import Oqarina.aadl_declarative.
-Require Import Oqarina.aadl_thread_properties.
+
 Require Import Oqarina.aadl_communication_properties.
+Require Import Oqarina.aadl_thread_properties.
+Require Import Oqarina.aadl_timing_properties.
+
 Require Import Oqarina.aadl_aadl_project.
 Require Import Oqarina.aadl_feature_helper.
+
+Open Scope Z_scope.
 (* end hide *)
 
 (** ** Port Variable *)
@@ -34,18 +39,27 @@ Require Import Oqarina.aadl_feature_helper.
 (**
 Port variable maps AADL features to runtime level entities. Since we use Coq to define the dynamic semantics of AADL, it is also reasonnable to define the concept of port variable and use it to capture further the dynamic semantics of AADL threads.
 
- %\paragraph{}\define{Port Variable (AADLv2.2 \S 8.2)}{Port Variable (AADL)}{A port variable captures the feature at runtime. It implements runtime services to interact with the feature.}%
+ %\paragraph{}\define{Port Variable (AADLv2.2 \S 8.2)}{Port Variable (AADL)}{A port variable captures the feature of a component as a runtime entity. Port variables are accessed through runtime services.}%
 
-A port variable is captured using a Coq record. We define the concept of invalid port variable and a constructor for this record, along with the well-formedness rule and decidability result.
+A port variable is modeled by a Coq record. We define the concept of invalid port variable and a constructor for this record, along withe well-formedness rule and decidability result.
 *)
 
-Open Scope Z_scope.
+Module PortVal.
+  Definition V := prod AADL_Time bool.
+End PortVal.
+Module PortQueue := ListQueue PortVal.
 
 (* begin hide *)
 Section Port_Variable.
 (* end hide *)
 
-  Definition Port_Queue : Type := ListQueue.queue.
+  Definition Port_Queue : Type := PortQueue.queue.
+  Lemma Port_Queue_dec : forall x y : Port_Queue, {x=y}+{x<>y}.
+  Proof.
+    repeat decide equality.
+  Qed.
+
+  (** A [port_variable] has a reference to an AADL feature, a queue that stores incoming events or calls. A port variable also has a [port_input_times] that indicates when a feature can be frozen, and an urgency value to discriminate among activated triggering features. *)
 
   Record port_variable : Type := {
     port : feature;
@@ -54,25 +68,32 @@ Section Port_Variable.
     urgency : Z;
   }.
 
+  (* begin hide *)
   Lemma port_variable_eq_dec : forall x y : port_variable, {x=y}+{x<>y}.
   Proof.
     decide equality.
     apply Z.eq_dec. (*PeanoNat.Nat.eq_dec.*)
     apply input_time_eq_dec.
-    apply list_eq_dec; apply bool_dec.
+    apply Port_Queue_dec.
     apply feature_eq_dec.
   Defined.
+  (* end hide *)
+
+  (** [mkPortVariable] maps an AADL feature to a [port_variable]. The port variable is initialized with an empty queue. XXX default for port_input_time to be adjusted *)
 
   Definition mkPortVariable (f : feature) := {|
     port := f;
     variable := [];
-    port_input_times := Input_Time [ Default_IO_Time_Spec ]; (* XXX default value to change*)
-    urgency := 0;
+    port_input_times := Input_Time [ Default_IO_Time_Spec ];
+    urgency := Map_Urgency (projectionFeatureProperties f);
   |}.
+
+  (** A port variable is well-formed iff its configuration parameters are well-formed. This property is decidable. *)
 
   Definition port_variable_wf (p : port_variable) :=
     input_time_wf p.(port_input_times).
 
+  (* begin hide *)
   Definition port_variable_wf_dec : forall p : port_variable,
     dec_sumbool (port_variable_wf p).
   Proof.
@@ -81,17 +102,18 @@ Section Port_Variable.
     destruct port_input_times.
     apply input_time_wf_dec.
   Defined.
+  (* end hide *)
 
   Definition Invalid_Port_Variable := mkPortVariable Invalid_Feature.
 
   Definition Update_Variable (p : port_variable) (v : Port_Queue): port_variable := {|
     port := p.(port);
     variable := v;
-    port_input_times := p.( port_input_times);
+    port_input_times := p.(port_input_times);
     urgency := p.(urgency);
   |}.
 
-(** [Build_Input_Port_Variables] (resp. [Build_Output_Port_Variables]) is a utility functions that builds port variables from input (resp. output) features. \change{what about inout?} *)
+  (** [Build_Input_Port_Variables] (resp. [Build_Output_Port_Variables]) is a utility function that builds port variables from input (resp. output) features. AADL inout features are also considered. *)
 
   Definition Build_Input_Port_Variables (l : list feature) :=
     map mkPortVariable (Get_Input_Features l).
@@ -110,6 +132,7 @@ End Port_Variable.
 (* begin hide*)
 Section Thread_State_Variable.
 (* end hide *)
+
 (** [Build_Dispatch_Trigger] returns the list of triggering features *)
 
   Definition Build_Dispatch_Trigger (l : list feature) :=
@@ -122,8 +145,8 @@ TBD
   Record thread_state_variable : Type := {
     dispatch_protocol : Dispatch_Protocol;
     period : AADL_Time;
-  (*  deadline : AADL_Time;
-    wcet : AADL_Time; *)
+    deadline : AADL_Time;
+   (* wcet : AADL_Time; *)
     priority : Z;
     clock : AADL_Time;
     input_ports : list port_variable;
@@ -135,6 +158,7 @@ TBD
     dispatch_protocol := Map_Scheduling_Protocol (t->properties);
     period := Map_Period (t->properties);
     priority := Map_Priority (t->properties);
+    deadline := Map_Deadline (t->properties);
     clock := 0;
     input_ports := Build_Input_Port_Variables (t->features);
     output_ports := Build_Output_Port_Variables (t->features);
@@ -155,13 +179,14 @@ Section AADL_Dispatching.
 
 (** *** Intermediate Predicates
 
-Most dispatch protocols review the state of triggering features. We build the [Thread_Has_Activated_Triggering_Feature] predicate as a conjunction of more basic predicates,  in [Prop], and demonstrate their decidability.
+All AADL dispatch protocols review the state of triggering features and the current clock. We build the [Thread_Has_Activated_Triggering_Feature] predicate as a conjunction of more basic predicates, in [Prop], and demonstrate their decidability.
 
-First, we check whether the feature is activated, [Is_Feature_Activiated], then whether it is in the dispatch trigger, in [Feature_In_Dispatch_Trigger]. *)
+First, we check whether the feature is activated, [Is_Feature_Activated], then whether it is in the dispatch trigger, in [Feature_In_Dispatch_Trigger]. *)
 
   Definition Is_Feature_Activated (p : port_variable) :=
-    ~ ListQueue.Is_Empty p.(variable).
+    ~ PortQueue.Is_Empty p.(variable).
 
+  (* begin hide *)
   Lemma Is_Feature_Activated_dec :
     forall (p : port_variable), dec_sumbool (Is_Feature_Activated p).
   Proof.
@@ -169,12 +194,14 @@ First, we check whether the feature is activated, [Is_Feature_Activiated], then 
     unfold dec_sumbool.
     unfold Is_Feature_Activated.
     apply dec_sumbool_not.
-    apply ListQueue.Is_Empty_dec.
+    apply PortQueue.Is_Empty_dec.
   Defined.
+  (* end hide *)
 
   Definition Feature_In_Dispatch_Trigger (p : port_variable) (d : list feature) :=
     In p.(port) d.
 
+  (* begin hide *)
   Definition Feature_In_Dispatch_Trigger_dec :
     forall (p : port_variable) (d : list feature),
       dec_sumbool (Feature_In_Dispatch_Trigger p d).
@@ -185,12 +212,14 @@ First, we check whether the feature is activated, [Is_Feature_Activiated], then 
     apply In_dec.
     apply feature_eq_dec.
   Defined.
+  (* end hide *)
 
-  (** From that point, we can build [Thread_Has_Activated_Triggering_Feature] that is true iff. the thread has at least one activated triggering feature (predicate [Is_Activated_Triggering_Feature]). *)
+  (** From that point, we can build [Thread_Has_Activated_Triggering_Feature] that is true iff. the thread has at least one activated triggering feature that is also in the dispatch trigger. *)
 
   Definition Is_Activated_Triggering_Feature (p : port_variable)  (d : list feature) :=
     Is_Feature_Activated p /\ Feature_In_Dispatch_Trigger p d.
 
+  (* begin hide *)
   Lemma Is_Activated_Triggering_Feature_dec:
     forall (p : port_variable)  (d : list feature),
       dec_sumbool (Is_Activated_Triggering_Feature p d).
@@ -201,14 +230,12 @@ First, we check whether the feature is activated, [Is_Feature_Activiated], then 
     apply Is_Feature_Activated_dec.
     apply Feature_In_Dispatch_Trigger_dec.
   Defined.
+  (* end hide *)
 
-  Fixpoint Has_Activated_Triggering_Feature (l : list port_variable) (d : list feature) :=
-    match l with
-      | nil => False
-      | h :: t => Is_Activated_Triggering_Feature h d \/
-                  Has_Activated_Triggering_Feature t d
-    end.
+  Definition Has_Activated_Triggering_Feature (l : list port_variable) (d : list feature) :=
+    All_Or (fun x => (Is_Activated_Triggering_Feature x d)) l.
 
+  (* begin hide *)
   Lemma Has_Activated_Triggering_Feature_dec :
     forall (l : list port_variable) (d : list feature),
       dec_sumbool (Has_Activated_Triggering_Feature l d).
@@ -218,15 +245,17 @@ First, we check whether the feature is activated, [Is_Feature_Activiated], then 
     unfold Has_Activated_Triggering_Feature.
     induction l.
     - auto.
-    - apply dec_sumbool_or.
+    - unfold All_Or. apply dec_sumbool_or.
       * apply Is_Activated_Triggering_Feature_dec.
       * apply IHl.
   Defined.
+  (* end hide *)
 
   Definition Thread_Has_Activated_Triggering_Feature (th : thread_state_variable) :=
     Has_Activated_Triggering_Feature
       th.(input_ports) th.(dispatch_trigger).
 
+  (* begin hide *)
   Lemma Thread_Has_Activated_Triggering_Feature_dec :
     forall (th : thread_state_variable),
       dec_sumbool (Thread_Has_Activated_Triggering_Feature th).
@@ -237,14 +266,16 @@ First, we check whether the feature is activated, [Is_Feature_Activiated], then 
     intros.
     apply Has_Activated_Triggering_Feature_dec.
   Defined.
+(* end hide *)
 
 (** *** Definition of [Enabled]
 
-From the previous definitions, we can now define the [Enabled] function that returns [true] when a thread is dispatched.  *)
+From the previous definitions, we can now define the [Enabled] function that returns [true] when a thread is dispatched. First, we define basic predicates for each dispatch protocol.*)
 
   Definition Periodic_Enabled (th : thread_state_variable) :=
     th.(clock) mod th.(period) = 0.
 
+  (* begin hide *)
   Lemma Periodic_Enabled_dec:
     forall (th : thread_state_variable), dec_sumbool (Periodic_Enabled th).
   Proof.
@@ -253,10 +284,12 @@ From the previous definitions, we can now define the [Enabled] function that ret
     intros.
     apply Z.eq_dec.
   Defined.
+  (* end hide *)
 
   Definition Aperiodic_Enabled (th : thread_state_variable) :=
     Thread_Has_Activated_Triggering_Feature th.
 
+  (* begin hide *)
   Lemma Aperiodic_Enabled_dec:
     forall (th : thread_state_variable), dec_sumbool (Aperiodic_Enabled th).
   Proof.
@@ -265,11 +298,13 @@ From the previous definitions, we can now define the [Enabled] function that ret
     intros.
     apply Thread_Has_Activated_Triggering_Feature_dec.
   Defined.
+  (* end hide *)
 
   Definition Sporadic_Enabled (th : thread_state_variable) :=
     th.(period) <= th.(clock) /\
      Thread_Has_Activated_Triggering_Feature th.
 
+  (* begin hide *)
   Lemma Sporadic_Enabled_dec:
     forall (th : thread_state_variable), dec_sumbool (Sporadic_Enabled th).
   Proof.
@@ -280,11 +315,13 @@ From the previous definitions, we can now define the [Enabled] function that ret
     apply Z_le_dec. (* {period th <= clock th} + {~ period th <= clock th} *)
     apply Thread_Has_Activated_Triggering_Feature_dec.
   Defined.
+  (* end hide *)
 
   Definition Timed_Enabled (th : thread_state_variable) :=
     (th.(period) = th.(clock)) \/
     Thread_Has_Activated_Triggering_Feature th.
 
+  (* begin hide *)
   Lemma Timed_Enabled_dec:
     forall (th : thread_state_variable), dec_sumbool (Timed_Enabled th).
   Proof.
@@ -295,11 +332,13 @@ From the previous definitions, we can now define the [Enabled] function that ret
     apply Z.eq_dec.
     apply Thread_Has_Activated_Triggering_Feature_dec.
   Defined.
+  (* end hide *)
 
   Definition Hybrid_Enabled (th : thread_state_variable) :=
     (th.(period) = th.(clock)) /\
     Thread_Has_Activated_Triggering_Feature th.
 
+  (* begin hide *)
   Lemma Hybrid_Enabled_dec:
     forall (th : thread_state_variable), dec_sumbool (Hybrid_Enabled th).
   Proof.
@@ -310,10 +349,12 @@ From the previous definitions, we can now define the [Enabled] function that ret
     apply Z.eq_dec.
     apply Thread_Has_Activated_Triggering_Feature_dec.
   Defined.
+  (* end hide *)
 
   Definition Background_Enabled (th : thread_state_variable) :=
     True.
 
+  (* begin hide *)
   Lemma Background_Enabled_dec:
     forall (th : thread_state_variable), dec_sumbool (Background_Enabled th).
   Proof.
@@ -321,6 +362,9 @@ From the previous definitions, we can now define the [Enabled] function that ret
     unfold Background_Enabled.
     auto.
   Defined.
+  (* end hide *)
+
+  (** Then we define the [Enabled] predicate *)
 
   Definition Enabled (th : thread_state_variable) :=
     match th.(dispatch_protocol) with
@@ -333,6 +377,7 @@ From the previous definitions, we can now define the [Enabled] function that ret
     | Unspecified => False
     end.
 
+  (* begin hide *)
   Lemma Enabled_dec: forall (th : thread_state_variable), dec_sumbool (Enabled th).
   Proof.
     unfold dec_sumbool.
@@ -347,11 +392,12 @@ From the previous definitions, we can now define the [Enabled] function that ret
     apply Timed_Enabled_dec.
     apply Hybrid_Enabled_dec.
   Defined.
+  (* end hide *)
 
-  (** [Enabled_oracle] return a [bool] as a witness, useful only for debugging purposes. *)
+  (** [Enabled_oracle] return a [bool] as a witness, for debugging purposes. *)
+
   Definition Enabled_oracle (th : thread_state_variable) :=
     Oracle (Enabled_dec th).
-  (*  if Enabled_dec th then true else false.*)
 
 (* begin hide *)
 End AADL_Dispatching.
@@ -359,18 +405,12 @@ End AADL_Dispatching.
 
 (** ** Ports Queue Processing *)
 
-(**  The following is a first cut at formalizing ports from %\S 8.3%. We capture the definition of [Frozen] for ports. *)
+(**  The following is a first cut at formalizing ports from %\S 8.3%. We capture the definition of [Frozen] for ports. First, we build ATF, the list of Activated Triggering Features. *)
 
 (** [Activated_Triggering_Features] returns the list of Activated Triggering Features. *)
 
-Fixpoint Activated_Triggering_Features' (l : list port_variable) (d : list feature) :=
-  match l with
-  | nil => nil
-  | h :: t => match Is_Activated_Triggering_Feature_dec h d with
-                  | left _=> h :: (Activated_Triggering_Features' t d)
-                  | right _ => Activated_Triggering_Features' t d
-              end
-  end.
+Definition Activated_Triggering_Features'  (l : list port_variable) (d : list feature) :=
+  filter (fun x => Oracle (Is_Activated_Triggering_Feature_dec x d) ) l.
 
 Definition Activated_Triggering_Features (th : thread_state_variable) :=
   Activated_Triggering_Features' th.(input_ports) th.(dispatch_trigger).
@@ -379,14 +419,14 @@ Definition Activated_Triggering_Features (th : thread_state_variable) :=
 
 Fixpoint Get_Port_Variable_With_Max_Urgency
   (p : port_variable) (l : list port_variable) : port_variable :=
-  match l with
-  | nil => p
-  | h :: t => if p.(urgency) <=? h.(urgency) then
-      Get_Port_Variable_With_Max_Urgency h t else
-      Get_Port_Variable_With_Max_Urgency p t
-    (* note we take h in all cases, this is to address the case where the
-       first argument is [Invalid_Feature] *)
-  end.
+    match l with
+    | nil => p
+    | h :: t => if p.(urgency) <=? h.(urgency) then
+        Get_Port_Variable_With_Max_Urgency h t else
+        Get_Port_Variable_With_Max_Urgency p t
+      (* note we take h in all cases, this is to address the case where the
+        first argument is [Invalid_Port_Variable] *)
+    end.
 
 (** Then, we can define the [Get_Elected_Triggering_Feature] that returns the elected features among Activated Triggering Features. XXX must define this concept in the standard. *)
 
@@ -405,7 +445,9 @@ Definition Dispatch_Frozen (p : port_variable) (th : thread_state_variable) : Pr
    (p = Get_Elected_Triggering_Feature  th) \/
        ~ (Feature_In_Dispatch_Trigger p th.(dispatch_trigger)).
 
-Definition Dispatch_Frozen_dec: forall p th, { Dispatch_Frozen p th } + { ~ Dispatch_Frozen p th }.
+(* begin hide *)
+Definition Dispatch_Frozen_dec:
+  forall p th, { Dispatch_Frozen p th } + { ~ Dispatch_Frozen p th }.
 Proof.
   intros.
   unfold Dispatch_Frozen.
@@ -414,6 +456,7 @@ Proof.
   apply dec_sumbool_not.
   apply Feature_In_Dispatch_Trigger_dec.
 Defined.
+(* end hide *)
 
 Definition Frozen (p : port_variable) (th : thread_state_variable) : Prop :=
   match Current_Valid_IO_Time_Spec p th with
@@ -434,45 +477,70 @@ Section Thread_RTS.
 
 (** A collection of runtime services is provided. A runtime service manipulates the thread state and its assocoated port variable *)
 
-(** %\define{Advance time (Coq)}{advance\_time (Coq)}
-{TBD}
+(** %\define{advance\_time (Coq)}{advance\_time (Coq)}
+{$advance\_time(th, t)$ increments the clock of the thread state variable:\\
+  $$\infer[advance\_time(th, t)]{th() \rightarrow th (clock \leftarrow clock + t)}{th, t \geq 0}$$
+}
    %*)
 
-  Definition advance_time (t : thread_state_variable) (tt : AADL_Time): thread_state_variable := {|
-    dispatch_protocol := t.(dispatch_protocol);
-    period := t.(period);
-    priority := t.(priority);
-    clock := t.(clock) + tt;
-    input_ports := t.(input_ports);
-    output_ports := t.(output_ports);
-    dispatch_trigger := t.(dispatch_trigger);
-  |}.
+  Definition advance_time (th : thread_state_variable) (t : AADL_Time) := {|
+      dispatch_protocol := th.(dispatch_protocol);
+      period := th.(period);
+      deadline := th.(deadline);
+      priority := th.(priority);
+      clock := th.(clock) + t;
+      input_ports := th.(input_ports);
+      output_ports := th.(output_ports);
+      dispatch_trigger := th.(dispatch_trigger);
+    |}.
 
 (** %\begin{definition}[store\_in (Coq)]
 TBD
   \end{definition} %*)
 
-  Definition Store_In_ (p : port_variable) (name : identifier) (value : bool) :=
+  Definition Store_In_ (p : port_variable) (name : identifier) (value : PortVal.V) :=
     if identifier_beq (projectionFeatureIdentifier p.(port)) name then
-      Update_Variable p (ListQueue.enq p.(variable) value)
+      Update_Variable p (PortQueue.enq p.(variable) value)
     else
       p.
 
-  Fixpoint Store_In (l : list port_variable) (name : identifier) (value : bool) :=
+  Fixpoint Store_In (l : list port_variable) (name : identifier) (value : PortVal.V) :=
     match l with
     | nil => l
     | h :: t => Store_In_ h name value :: Store_In t name value
     end.
 
-  Definition store_in (t : thread_state_variable) (name : identifier) (value : bool) : thread_state_variable := {|
+  Definition store_in (t : thread_state_variable) (name : identifier) (value : bool) := {|
     dispatch_protocol := t.(dispatch_protocol);
     period := t.(period);
+    deadline := t.(deadline);
     priority := t.(priority);
     clock := t.(clock);
-    input_ports := Store_In t.(input_ports) name value;
+    input_ports := Store_In t.(input_ports) name (t.(clock), value);
     output_ports := t.(output_ports);
     dispatch_trigger := t.(dispatch_trigger);
   |}.
+
+(** %\begin{definition}[Get\_Count (Coq)]
+TBD
+  \end{definition} %*)
+
+  Definition Get_Count_ (p : port_variable) (name : identifier) :=
+    if identifier_beq (projectionFeatureIdentifier p.(port)) name then
+      PortQueue.count p.(variable)
+    else
+      0%nat.
+
+  (** XXX Ugly implementaiton, should probably filter and then count. It basically works because there is unicity of port variable names *)
+
+  Fixpoint Get_Count (l : list port_variable) (name : identifier) : nat :=
+    match l with
+    | nil => 0%nat
+    | h :: t => Get_Count_ h name + Get_Count t name
+    end.
+
+  Definition get_count (t : thread_state_variable) (name : identifier) :=
+    Get_Count t.(input_ports) name.
 
 (* begin hide *)
 End Thread_RTS.
@@ -494,7 +562,7 @@ Definition A_Priority_Value := {|
 
 Definition A_Period := {|
   PT := PT_TypeRef (Period_Name);
-  PV := PV_Int 3;
+  PV := PV_IntU 3 (PV_Unit (Id "ms"));
 |}.
 
 Definition A_Periodic_Thread := Component
@@ -508,16 +576,18 @@ Definition A_Periodic_Thread := Component
 Definition A_Periodic_Thread_State := mk_thread_state_variable (A_Periodic_Thread).
 
 (** At t = 0, the periodic thread is enabled *)
-Compute Enabled_oracle (A_Periodic_Thread_State).
-(*
-	 = true
-     : bool
-*)
+Lemma Periodic_t0_enabled :  Enabled_oracle (A_Periodic_Thread_State) = true.
+Proof.
+  trivial.
+Qed.
 
 Definition A_Periodic_Thread_State' := advance_time A_Periodic_Thread_State 4.
 
 (** At t = 4, the periodic thread is not enabled *)
-Compute Enabled_oracle (A_Periodic_Thread_State').
+Lemma Periodic_t4_not_enabled : Enabled_oracle (A_Periodic_Thread_State') = false.
+Proof.
+  trivial.
+Qed.
 
 (** *** A Sporadic Thread*)
 
@@ -543,18 +613,34 @@ Definition A_Sporadic_Thread := Component
 Definition A_Sporadic_Thread_State := mk_thread_state_variable (A_Sporadic_Thread).
 
 (** initially, the sporadic thread is not enabled *)
-Eval vm_compute in Enabled_oracle (A_Sporadic_Thread_State).
+Lemma Sporatic_tO_not_enabled : Enabled_oracle (A_Sporadic_Thread_State) = false.
+Proof.
+  trivial.
+Qed.
 
 (** inject en event *)
 Definition A_Sporadic_Thread_State' := store_in A_Sporadic_Thread_State (Id "a_feature") true.
 
 (** the thread is not enabled yet *)
-Compute Enabled_oracle (A_Sporadic_Thread_State').
+Lemma Sporatic_tO_not_enabled' : Enabled_oracle (A_Sporadic_Thread_State') = false.
+Proof.
+  trivial.
+Qed.
 
 (** we advance time *)
 Definition th := advance_time A_Sporadic_Thread_State' 32.
 
 (** the thread is enabled, and we can check frozen port *)
-Compute Enabled_oracle th.
+Lemma Sporadic_t42_enabled : Enabled_oracle th = true.
+Proof.
+  trivial.
+Qed.
+
 Compute Get_Elected_Triggering_Feature (th).
+
 Compute Frozen_Ports' (th).
+
+Lemma get_count_1 : get_count th (Id "a_feature") = 1%nat.
+Proof.
+  trivial.
+Qed.
