src/coq_utils/utils.v
@@ -18,13 +18,19 @@ Set Implicit Arguments.
 Section All.
 (* end hide *)
 
-    Variable T : Set.
+    Variable T : Type.
     Variable P : T -> Prop.
 
     Fixpoint All (ls : list T) : Prop :=
       match ls with
         | nil => True
         | h :: t => P h /\ All t
+      end.
+
+    Fixpoint All_Or (ls : list T) : Prop :=
+      match ls with
+        | nil => False
+        | h :: t => P h \/ All_Or t
       end.
 
     (** We show that if %\coqdocvar{HP}% holds, then %\coqdocvar{All}%
@@ -37,6 +43,15 @@ Section All.
       induction lt.
       - unfold All. apply dec_True. (* from Coq.Logic.Decidable *)
       - simpl. apply dec_and. (* from Coq.Logic.Decidable *)
+        * apply HP.
+        * apply IHlt.
+    Qed.
+
+    Lemma All_Or_dec: forall lt : list T, decidable(All_Or lt).
+    Proof.
+      induction lt.
+      - unfold All_Or. apply dec_False. (* from Coq.Logic.Decidable *)
+      - simpl. apply dec_or. (* from Coq.Logic.Decidable *)
         * apply HP.
         * apply IHlt.
     Qed.
