src/aadl_timing_properties.v
@@ -1,29 +1,84 @@
-(** %\chapter{\texttt{AADL\_Project}} %*)
+(** %\chapter{\texttt{Timing\_Properties}} %*)
 
 (** Loose mapping of aadl_project.aadl to define common types, units, etc. *)
 
+(* begin hide *)
+(** Coq Library *)
 Require Import Coq.Lists.List.
 Import ListNotations.
+Require Import Coq.ZArith.ZArith.
 
+(** Oqarina library *)
 Require Import Oqarina.core.identifiers.
 Require Import Oqarina.core.time.
 Require Import Oqarina.properties.properties.
-
 Require Import Oqarina.aadl_aadl_project.
+Require Import Oqarina.aadl_categories.
+(* end hide *)
+
+(** ** %\texttt{timing\_properties}% as Coq/AADL property_types *)
 
 Definition Timing_Properties_PS :=
     PropertySet (Id "Timing_Properties") [
 
     (* Time: type aadlinteger 0 ps .. Max_Time units Time_Units; *)
 
-    "Time" :prop PT_Number aadlinteger None (Some (PT_TypeRef (PSQN "AADL_Project_PS" "Time_Units"))) => None
-       applies [];
+    "Time" :prop PT_Number aadlinteger None (Some (PT_TypeRef (PSQN "AADL_Project_PS" "Time_Units")))
+      => None applies [];
+
+    (* Deadline: inherit Time => Period
+		   applies to (thread, thread group, process, system, device, virtual processor);
+    *)
+
+    "Deadline" :prop PT_TypeRef (PSQN "Timing_Properties" "Time")
+        => None applies [ thread ; threadGroup ; process ; system ; device ; virtualProcessor];
 
     (* Period: inherit Time
        applies to (thread, thread group, process, system, device, virtual processor);
     *)
 
     "Period" :prop PT_TypeRef (PSQN "Timing_Properties" "Time")
-        => None applies []
+        => None applies [ thread ; threadGroup ; process ; system ; device ; virtualProcessor]
   ].
 
+(*
+%\paragraph{} \begin{definition}[Period (\S XXX]
+ TBD
+  \end{definition}% *)
+
+Definition Period_Name := PSQN "timing_properties" "period".
+
+Definition Is_Period (pa : property_association) :=
+  Is_Property_Name Period_Name pa.
+
+(*
+%\paragraph{} \begin{definition}[Deadline (\S XXX]
+ TBD
+  \end{definition}% *)
+
+  Definition Deadline_Name := PSQN "timing_properties" "deadline".
+
+  Definition Is_Deadline (pa : property_association) :=
+    Is_Property_Name Deadline_Name pa.
+
+(**
+
+%
+  \begin{definition}[Period (Coq)]
+  TBD
+  \end{definition}
+% *)
+
+Definition Map_Period (pa : list property_association) : Z :=
+  Map_PV_Int_List pa Is_Period.
+
+(**
+
+%
+  \begin{definition}[Deadline (Coq)]
+  TBD
+  \end{definition}
+% *)
+
+Definition Map_Deadline (pa : list property_association) : Z :=
+  Map_PV_Int_List pa Is_Deadline.
